certicoq/Makefile
@@ -1,7 +1,7 @@
 
 all: theories/Makefile libraries/Makefile
 	$(MAKE) -C libraries
-	$(MAKE) -C libraries/SquiggleEq
+#	$(MAKE) -C libraries/SquiggleEq
 	$(MAKE) -C theories
 	
 
@@ -13,8 +13,13 @@ libraries/Makefile:
 
 clean:
 	$(MAKE) clean -C libraries
-	$(MAKE) clean -C libraries/SquiggleEq
+#	$(MAKE) clean -C libraries/SquiggleEq
 	$(MAKE) clean -C theories
+
+cleanCoqc:
+	find -name *.vo | xargs rm
+	find -name *.glob | xargs rm
+	find -name *.v.d | xargs rm
 	
 gitsuperclean:
 	git reset HEAD --hard
